theories/lang/notation.v
@@ -150,9 +150,7 @@ Definition void_layout : layout := {| ly_size := 0; ly_align_log := 0 |}.
 Definition void_ptr : layout := {| ly_size := bytes_per_addr; ly_align_log := bytes_per_addr_log |}.
 Notation "'void*'" := (void_ptr).
 
-Definition NULL : val := i2v 0 size_t.
 Definition VOID : val := [].
-Typeclasses Opaque NULL.
 
 Definition field_list := list (option var_name * layout).
 
